Finish DependentlyTypedSum combinator for RDP

src/Common/Equality.v
@@ -1,6 +1,7 @@
 Require Import Coq.Lists.List.
 
 Set Implicit Arguments.
+Local Close Scope nat_scope.
 
 Definition pr1_path {A} {P : A -> Type} {u v : sigT P} (p : u = v)
 : projT1 u = projT1 v
@@ -66,3 +67,48 @@ Section option.
   Definition Some_injective {x y : A} : Some x = Some y -> x = y
     := option_encode.
 End option.
+
+Section sum.
+  Context {A B : Type}.
+
+  Definition sum_code (x y : A + B) : Prop
+    := match x, y with
+         | inl x', inl y' => x' = y'
+         | inr x', inr y' => x' = y'
+         | _, _ => False
+       end.
+
+  Definition sum_code_idpath {x} : sum_code x x
+    := match x return sum_code x x with
+         | inl _ => eq_refl
+         | inr _ => eq_refl
+       end.
+
+  Definition sum_encode {x y} (p : x = y) : sum_code x y
+    := eq_rect _ _ sum_code_idpath _ p.
+
+  Definition sum_decode {x y} : sum_code x y -> x = y
+    := match x, y return sum_code x y -> x = y with
+         | inl x', inl y' => @f_equal _ _ (@inl _ _) _ _
+         | inr x', inr y' => @f_equal _ _ (@inr _ _) _ _
+         | _, _ => fun H => match H : False with end
+       end.
+
+  Definition sum_deenecode {x y} (p : x = y)
+  : sum_decode (sum_encode p) = p.
+  Proof.
+    destruct p, x; reflexivity.
+  Defined.
+
+  Definition sum_endecode {x y} (p : sum_code x y)
+  : sum_encode (sum_decode p) = p.
+  Proof.
+    destruct x, y, p; reflexivity.
+  Defined.
+
+  Definition inl_injective {x y : A} : inl x = inl y -> x = y
+    := sum_encode.
+
+  Definition inr_injective {x y : B} : inr x = inr y -> x = y
+    := sum_encode.
+End sum.
